src/named/IExp.v
@@ -14,7 +14,7 @@ Inductive exp : Set :=
 (* Rule label, list of subterms*)
 | con : string -> list exp -> exp
 | ann : exp -> sort -> exp                         
-with sort : Set := srt : string -> list exp -> sort.
+with sort : Set := scon : string -> list exp -> sort.
 Set Elimination Schemes.
 
 
@@ -27,7 +27,7 @@ Definition subst_lookup (s : subst) (n : string) : exp :=
 Global Transparent subst_lookup.
 
 Definition ctx_lookup (c: ctx) (n : string) : sort :=
-  named_list_lookup (srt "" [::]) c n.
+  named_list_lookup (scon "ERR" [::]) c n.
 Global Transparent ctx_lookup.
 
 (*TODO: move to utils*)
@@ -45,7 +45,7 @@ Fixpoint exp_var_map (f : string -> exp) (e : exp) : exp :=
   end
 with sort_var_map f t :=
        match t with
-       | srt n s => srt n (map (exp_var_map f) s)
+       | scon n s => scon n (map (exp_var_map f) s)
        end.
 
 Definition exp_subst (s : subst) e : exp :=
@@ -89,7 +89,7 @@ by rewrite subst_subst_assoc.
 Defined.
 
 Definition sort_subst (s : subst) (t : sort) : sort :=
-  let (c, s') := t in srt c (map (apply_subst s) s').
+  let (c, s') := t in scon c (map (apply_subst s) s').
 
 Lemma sort_subst_assoc : forall s1 s2 a,
     sort_subst s1 (sort_subst s2 a)
@@ -101,3 +101,127 @@ Instance substable_sort : Substable sort :=
   apply_subst := sort_subst;
   subst_assoc := sort_subst_assoc;
   }.
+
+Module Notations.
+
+  Declare Custom Entry exp.
+  Declare Custom Entry sort.
+  
+
+  Declare Custom Entry ctx.
+  Declare Custom Entry ctx_binding.
+
+  (* Since contexts are regular lists, 
+     we need a scope to determine when to print them *)
+  Declare Scope ctx_scope.
+  Bind Scope ctx_scope with ctx.
+
+  (* for notation purposes *)
+  Definition as_ctx (c : ctx) := c.
+  
+  Notation "'{{e' e }}" := (e) (at level 0,e custom exp at level 100).
+  Notation "'{{s' e }}" := (e) (at level 0,e custom sort at level 100).
+  Notation "'{{c' e }}" := (as_ctx e) (at level 0,e custom ctx at level 100).
+  
+  Notation "{ x }" :=
+    x (in custom exp at level 0, x constr).
+  Notation "{ x }" :=
+    x (in custom sort at level 0, x constr).
+  (* TODO: issues; fix *)
+  Notation "{ x }" :=
+    x (in custom ctx at level 0, x constr).
+  
+  Notation "# c" :=
+    (con c%string [::])
+      (right associativity,in custom exp at level 0, c constr at level 0,
+                              format "# c").
+  Notation "# c" :=
+    (scon c%string [::])
+      (right associativity,in custom sort at level 0, c constr at level 0,
+                              format "# c").
+
+  Definition exp_constr_app e e' :=
+    match e with
+    | con c l => con c (e'::l)
+    | _ => con "ERR" [::]
+    end.
+
+  Definition srt_constr_app t e' :=
+    match t with
+    | scon c l => scon c (e'::l)
+    end.
+
+  Notation "c e" :=
+    (exp_constr_app c e)
+      (left associativity, in custom exp at level 10,
+                              c custom exp, e custom exp at level 9).
+  Notation "c e" :=
+    (srt_constr_app c e)
+      (left associativity, in custom sort at level 10,
+                              c custom sort, e custom exp at level 9).
+
+  Notation "( e )" := e (in custom exp at level 0, e custom exp at level 100).
+  Notation "( e )" := e (in custom sort at level 0, e custom sort at level 100).
+
+  Notation "% x" :=
+    (var x%string)
+      (in custom exp at level 0, x constr at level 0, format "% x").
+
+
+  Check {{e #"foo" }}.
+  Check {{e #"foo" (#"bar" %"x") #"baz" %"y"}}.
+  Check {{s #"foo" }}.
+  Check {{s #"foo" (#"bar" %"x") #"baz" %"y"}}.
+
+  
+  Eval compute in {{e #"foo" (#"bar" %"x") #"baz" %"y"}}.
+  
+  Notation "# c e1 .. en"
+    := (con c (cons en .. (cons e1 nil) ..))
+      (left associativity,
+         in custom exp at level 10,
+            c constr at level 0,
+            e1 custom exp at level 9,
+            en custom exp at level 9,
+            only printing).
+
+  Notation "# c e1 .. en"
+    := (scon c (cons en .. (cons e1 nil) ..))
+      (left associativity,
+         in custom sort at level 10,
+            c constr at level 0,
+            e1 custom exp at level 9,
+            en custom exp at level 9,
+            only printing).
+  
+  Eval compute in {{e #"foo" (#"bar" %"x") #"baz" %"y"}}.
+  Eval compute in {{s #"foo" (#"bar" %"x") #"baz" %"y"}}.
+  Eval compute in {{s #"foo" }}.
+                               
+
+
+  Notation "bd , .. , bd'" :=
+    (cons bd' .. (cons bd nil)..)
+      (in custom ctx at level 100, bd custom ctx_binding at level 100,
+          format "'[hv' bd ,  '/' .. ,  '/' bd' ']'") : ctx_scope.
+
+  (* TODO: temporary holdover until { c } works*)
+  Notation "! c" :=
+    (c)
+      (in custom ctx at level 0,
+          c constr at level 0) : ctx_scope.
+
+  Notation "" := nil (*(@nil (string*sort))*) (in custom ctx at level 0) : ctx_scope.
+
+  Notation "x : t" :=
+    (x%string, t)
+      (in custom ctx_binding at level 100, x constr at level 0,
+          t custom sort at level 100).
+
+  Check {{c }}.
+  Check {{c "x" : #"env"}}.
+  Check {{c "x" : #"env", "y" : #"ty" %"x", "z" : #"ty" %"x"}}.
+
+  Check let c := {{c }} in {{c !c}}.
+
+End Notations.
