README.md
@@ -1,5 +1,5 @@
 #TODOs
 
-* determine whether wf_sort wanted in wf_args_cons constructor
 * determine whether there is an issue w/ current lax typing on le judgments
-* prune obsolete lemmas
+* fill admits in subst lemmas for IExp
+* fill admits (or remove lemmas) for identity operation in Tactics
